Automation working for all our examples.

src/Narcissus/Formats/Option.v
@@ -3,13 +3,14 @@ Require Import
         Fiat.Computation
         Fiat.Computation.Notations
         Fiat.Narcissus.Common.Specs
-        Fiat.Narcissus.Common.WordFacts.
+        Fiat.Narcissus.Common.WordFacts
+        Fiat.Narcissus.BaseFormats.
 
 Unset Implicit Arguments.
 Section Option.
 
   Context {sz : nat}.
-  Context {S : Type}.
+  Context {S VS VN : Type}.
   Context {T : Type}.
   Context {cache : Cache}.
   Context {cacheAddNat : CacheAdd cache nat}.
@@ -27,11 +28,121 @@ Section Option.
     : EncodeM (option S) T :=
     fun a_opt => If_Opt_Then_Else a_opt encode_Some (encode_None ()).
 
-  Definition option_decode
-             (decode_Some : DecodeM (S * T) T)
-             (decode_None : DecodeM (() * T) T)
+  Definition option_decode'
+             (decode_Some : DecodeM (VS * T) T)
+             (decode_None : DecodeM (VN * T) T)
              (b' : bool)
-    : DecodeM ((option S) * T) T :=
+    : DecodeM ((VS + VN) * T) T :=
+    (fun (b : T) (env : CacheDecode) =>
+       If b' Then
+          match decode_Some b env with
+          | Some (a, b, c) => Some ((inl a, b), c)
+          | None => None
+          end
+          Else
+          match decode_None b env with
+          | Some (a, b, c) => Some ((inr a, b), c)
+          | None => None
+          end).
+
+  Lemma option_format_correct'
+      {P  : CacheDecode -> Prop}
+      {P_invT P_invE : (CacheDecode -> Prop) -> Prop}
+      (P_inv_pf : cache_inv_Property P (fun P => P_invT P /\ P_invE P))
+      (Source_Predicate : option S -> Prop)
+      (Some_View_Predicate : VS -> Prop)
+      (None_View_Predicate : VN -> Prop)
+      (viewS : S -> VS -> Prop)
+      (viewN : () -> VN -> Prop)
+      (b' : bool)
+      (predicate :=
+         fun a_opt =>
+           decides (negb b') (a_opt = None)
+           /\ Source_Predicate a_opt)
+      (format_Some : FormatM S T)
+      (format_None : FormatM () T)
+      (decode_Some : DecodeM (VS * T) T)
+      (decode_None : DecodeM (VN * T) T)
+      (view_format_Some : FormatM VS T)
+      (view_format_None : FormatM VN T)
+      (decode_Some_pf :
+         cache_inv_Property P P_invT
+         -> CorrectDecoder
+              monoid (fun s => Source_Predicate (Some s))
+              Some_View_Predicate
+              viewS
+              format_Some decode_Some P
+              view_format_Some)
+      (decode_None_pf :
+         cache_inv_Property P P_invE
+         -> CorrectDecoder
+              monoid
+              (fun _ => Source_Predicate None)
+              None_View_Predicate
+              viewN
+              format_None decode_None P
+              view_format_None)
+  : CorrectDecoder
+      monoid
+      predicate
+      (fun v_opt =>
+         match v_opt with
+         | inl vs => Some_View_Predicate vs /\ b' = true
+         | inr vn => None_View_Predicate vn /\ b' = false
+         end)
+      (fun s_opt v_opt =>
+         match s_opt, v_opt with
+         | Some s, inl vs => viewS s vs
+         | None, inr vn => viewN () vn
+         | _, _ => False
+         end)
+      (format_option format_Some format_None)
+      (option_decode' decode_Some decode_None b')
+      P (fun v_opt =>
+           match v_opt with
+           | inl vs => view_format_Some vs
+           | inr vn => view_format_None vn
+           end
+        ).
+Proof.
+  unfold cache_inv_Property in *; split.
+  { intros env env' xenv data bin ext ? env_pm pred_pm com_pf.
+    unfold format_option in com_pf; computes_to_inv;
+      unfold option_decode'; destruct data;
+      find_if_inside; unfold predicate in *; simpl in *;
+        intuition; try discriminate.
+    - eapply H3 in com_pf; destruct_ex;
+        subst; intuition eauto; rewrite H6; eauto.
+      subst; eexists _, _; eauto.
+    - eapply H4 in com_pf; destruct_ex;
+        intuition eauto; rewrite H6; eauto.
+      subst; eexists _, _; eauto.
+  }
+  { unfold option_decode'; intros.
+    find_if_inside; simpl in *.
+    - destruct (decode_Some t env') as [ [ [? ?] ?] | ] eqn : ? ;
+        simpl in *; try discriminate; injections; simpl.
+      eapply decode_Some_pf in Heqo; intuition eauto.
+      destruct_ex; split_and; eexists _, _; intuition eauto.
+    - destruct (decode_None t env') as [ [ [? ?] ?] | ] eqn : ? ;
+        simpl in *; try discriminate; injections.
+      eapply decode_None_pf in Heqo; intuition eauto; destruct_ex;
+        intuition eauto; subst.
+      destruct_ex; split_and; eexists _, _; intuition eauto.
+  }
+Qed.
+
+End Option.
+
+Definition option_decode
+           {S T}
+           {cache : Cache}
+           {cacheAddNat : CacheAdd cache nat}
+           (monoid : Monoid T)
+           (decode_Some : DecodeM (S * T) T)
+           (decode_None : DecodeM (() * T) T)
+           (b' : bool)
+    : DecodeM (option S * T) T :=
     (fun (b : T) (env : CacheDecode) =>
        If b' Then
           match decode_Some b env with
@@ -44,19 +155,23 @@ Section Option.
           | None => None
           end).
 
-  Lemma option_format_correct
-      {P  : CacheDecode -> Prop}
+Lemma option_format_correct
+      {S T}
+      {cache : Cache}
+      {cacheAddNat : CacheAdd cache nat}
+      (monoid : Monoid T)
+      {P : CacheDecode -> Prop}
       {P_invT P_invE : (CacheDecode -> Prop) -> Prop}
       (P_inv_pf : cache_inv_Property P (fun P => P_invT P /\ P_invE P))
-      (predicate_Some : S -> Prop)
-      (predicate_None : () -> Prop)
+      (Some_Predicate : S -> Prop)
+      (None_Predicate : Prop)
       (b' : bool)
       (predicate :=
          fun a_opt =>
            decides (negb b') (a_opt = None)
            /\ match a_opt with
-              | Some a => predicate_Some a
-              | None => predicate_None ()
+              | Some s => Some_Predicate s
+              | None => None_Predicate
               end)
       (format_Some : FormatM S T)
       (format_None : FormatM () T)
@@ -65,16 +180,19 @@ Section Option.
       (decode_Some_pf :
          cache_inv_Property P P_invT
          -> CorrectDecoder
-              monoid predicate_Some
-              predicate_Some
+              monoid
+              Some_Predicate
+              Some_Predicate
               eq
               format_Some decode_Some P
               format_Some)
       (decode_None_pf :
          cache_inv_Property P P_invE
          -> CorrectDecoder
-              monoid predicate_None predicate_None
-              eq
+              monoid
+              (fun _ => None_Predicate)
+              (fun _ => None_Predicate)
+              (fun u _ => True)
               format_None decode_None P
               format_None)
   : CorrectDecoder
@@ -83,36 +201,67 @@ Section Option.
       predicate
       eq
       (format_option format_Some format_None)
-      (option_decode decode_Some decode_None b')
-      P (format_option format_Some format_None).
-Proof.
-  unfold cache_inv_Property in *; split.
-  { intros env env' xenv data bin ext ? env_pm pred_pm com_pf.
-    unfold format_option in com_pf; computes_to_inv;
-      unfold option_decode; destruct data;
-      find_if_inside; unfold predicate in *; simpl in *;
-        intuition; try discriminate.
-    - eapply H3 in com_pf; destruct_ex;
-        subst; intuition eauto; rewrite H6; eauto.
-      subst; eexists _, _; eauto.
-    - eapply H4 in com_pf; destruct_ex;
-        intuition eauto; rewrite H6; eauto.
-      subst; eexists _, _; eauto.
-  }
-  { unfold option_decode; intros.
-    find_if_inside; simpl in *.
-    - destruct (decode_Some t env') as [ [ [? ?] ?] | ] eqn : ? ;
-        simpl in *; try discriminate; injections; simpl.
-      eapply decode_Some_pf in Heqo; intuition eauto.
-      destruct_ex; intuition; subst.
-      eexists _; eexists _; unfold predicate; intuition eauto.
-      discriminate.
-    - destruct (decode_None t env') as [ [ [? ?] ?] | ] eqn : ? ;
-        simpl in *; try discriminate; injections; destruct u.
-      eapply decode_None_pf in Heqo; intuition eauto; destruct_ex;
-        intuition eauto; subst.
-      eexists _; eexists _; unfold predicate; intuition eauto.
-  }
-Qed.
+      (option_decode monoid decode_Some decode_None b')
+      P
+      (format_option format_Some format_None).
+  Proof.
+    eapply format_decode_correct_alt.
+    2: instantiate (1 := predicate).
+    7: {
+      eapply injection_decode_correct
+        with (inj := fun v =>
+                       match v with
+                       | inl vs => Some vs
+                       | inr _ => None
+                       end).
+      eapply option_format_correct' with (b'0 := b')
+                                         (Source_Predicate :=
+                                            fun s => match s with
+                                                     | Some s => _ s
+                                                     | None => _
+                                                     end);
+        eauto.
+      - simpl; intros.
+        instantiate (1 := fun s v => match s with
+                                     | Some s => match v with
+                                                 | Some vs => s = vs
+                                                 | None => False
+                                                 end
+                                     | None => match v with
+                                               | Some vs => False
+                                               | None => True
+                                               end
+                                     end).
+        simpl; destruct s; destruct v; eauto.
+      - intros.
+        unfold predicate; destruct v; destruct b'; intuition eauto;
+          simpl; try congruence.
+      - intros.
+        instantiate (1 := fun v_opt => match v_opt with
+                            | Some vs => format_Some vs
+                            | _ => format_None ()
+                            end); simpl.
+        destruct v; eauto.
+        destruct u; apply unfold_computes; eauto.
+    }
+    - unfold flip, pointwise_relation; intros.
+      unfold predicate; intuition eauto.
+    - unfold flip, pointwise_relation, impl; intros.
+        unfold predicate in *; intuition eauto.
 
-End Option.
+    - unfold flip, pointwise_relation; intros; intuition eauto.
+      subst; destruct a0; eauto.
+      destruct a; destruct a0; intuition; try congruence.
+    - unfold flip, pointwise_relation; intros; intuition eauto.
+      unfold EquivFormat; intros; reflexivity.
+    - unfold flip, pointwise_relation; intros; intuition eauto.
+      unfold Compose_Decode, option_decode, option_decode'.
+      destruct b'; simpl.
+      destruct (decode_Some a a0) as [ [ [? ?] ?] | ]; simpl; eauto.
+      destruct (decode_None a a0) as [ [ [? ?] ?] | ]; simpl; eauto.
+    - unfold flip, pointwise_relation; intros; intuition eauto.
+      unfold EquivFormat; intros.
+      unfold format_option; destruct s; simpl.
+      reflexivity.
+      reflexivity.
+  Qed.
